theory/math/Order2.dfy
@@ -2,13 +2,15 @@
   Order stuff
 ******************************************************************************/
 
-module Order {
+module Order2 {
 
   // Any type T implementing Ord<T> must provide a predicate Lt(_,_)
   // and prove it behaves as _<_
   
-  trait {:ghost} Ord<T(==)> {
+  abstract module Ord {
 
+    type T
+ 
     // x < y
     ghost predicate Lt(x:T, y:T)  
 
@@ -42,69 +44,57 @@ module Order {
 
   // Implement Ord for nat
 
-  class {:ghost} NatOrd extends Ord<nat> {
+  module NatOrd refines Ord {
 
-    ghost predicate Lt(x:nat, y:nat) {
+    type T = nat
+
+    ghost predicate Lt(x:T, y:T) 
+    {
       x < y
     }
 
-    lemma lem_Lt_Irrfl(x:nat)
-      ensures !Lt(x, x)
+    lemma lem_Lt_Irrfl(x:T)
     { }
 
-    lemma lem_Lt_Trans(x:nat, y:nat, z:nat)
-      requires Lt(x, y) && Lt(y, z)
-      ensures  Lt(x, z)
+    lemma lem_Lt_Trans(x:T, y:T, z:T)
     { }
 
-    lemma lem_Lt_Antisym(x:nat, y:nat)
-      requires Lt(x, y)
-      ensures  !(Lt(y, x))  
-    { }  
+    lemma lem_Lt_Antisym(x:T, y:T)
+    { }      
 
-    lemma lem_Lt_NotEq(x:nat, y:nat)
-      requires Lt(x, y)
-      ensures  x != y    
+    lemma lem_Lt_NotEq(x:T, y:T)
     { }
 
-    lemma lem_Lt_IfNotEq(x:nat, y:nat)
-      requires x != y 
-      ensures  Lt(x, y) || Lt(y, x)   
+    lemma lem_Lt_IfNotEq(x:T, y:T)  
     { } 
 
-  }
+  }  
 
   // Implement Ord for real
 
-  class {:ghost} RealOrd extends Ord<real> {
+  module RealOrd refines Ord {
 
-    ghost predicate Lt(x:real, y:real) {
+    type T = real
+
+    ghost predicate Lt(x:T, y:T) 
+    {
       x < y
     }
 
-    lemma lem_Lt_Irrfl(x:real)
+    lemma lem_Lt_Irrfl(x:T)
       ensures !Lt(x, x)
     { }
 
-    lemma lem_Lt_Trans(x:real, y:real, z:real)
-      requires Lt(x, y) && Lt(y, z)
-      ensures  Lt(x, z)
+    lemma lem_Lt_Trans(x:T, y:T, z:T)
     { }
 
-    lemma lem_Lt_Antisym(x:real, y:real)
-      requires Lt(x, y)
-      ensures  !(Lt(y, x))  
+    lemma lem_Lt_Antisym(x:T, y:T)
     { }      
 
-
-    lemma lem_Lt_NotEq(x:real, y:real)
-      requires Lt(x, y)
-      ensures  x != y    
+    lemma lem_Lt_NotEq(x:T, y:T)
     { }
 
-    lemma lem_Lt_IfNotEq(x:real, y:real)
-      requires x != y 
-      ensures  Lt(x, y) || Lt(y, x)   
+    lemma lem_Lt_IfNotEq(x:T, y:T)
     { } 
 
   }  
