caseStudy/ADT/List/Impl/AppendAmortDAL.dfy
@@ -1,0 +1,54 @@
+include "../../../../theory/math/TypeR0.dfy"
+include "./DynaArrayList.dfy"
+include "./LemDynaArrayList.dfy"
+
+/******************************************************************************
+  Amortized analysis for Append in DynaArrayList
+******************************************************************************/
+
+module AppendAmortDAL {
+  
+  import opened TypeR0
+  import opened DynaArrayList
+  import opened LemDynaArrayList
+
+  // Cost of append
+  ghost function T(N:nat, C:nat, m:nat) : R0
+    requires N <= C
+  {
+    if N < C then Tappend2(N)    // = 1
+             else Tappend(m, N)  // = (m+1)*N + 1
+  }
+
+  // Cost sequence: cost at the state immediately before the i-th append:
+  ghost function c(i:nat, N:nat, C:nat, m:nat) : R0
+    requires N <= C
+  {
+    1.0 // TODO
+  }
+
+  // Cost over a sequence of n appends
+  method costSequence<T(0)>(al:DynaArrayList<T>, n:nat) returns (t:R0)
+    modifies al.Repr()
+    requires al.Valid()
+    requires n > 0
+    ensures al.Valid() && fresh(al.Repr() - old(al.Repr())) 
+  {
+    t := 0.0; 
+
+    for i := 1 to n+1
+      modifies al.Repr()
+      invariant al.Valid() && fresh(al.Repr() - old(al.Repr())) 
+    {
+      var N, m, C := al.Size(), al.m, al.Capacity();
+    label before:
+      var x:T :| true;
+      var t := al.Append(x);
+      assert t == if old@before(al.IsFull()) then Tappend(m, N) else Tappend2(N);
+      assert t == T(N, C, m);
+      
+      t := t + t;
+    }
+  }
+
+}
